Dfa.begin

Cslib/Computability/Dfa/Basic.lean
@@ -4,16 +4,67 @@ Released under Apache 2.0 license as described in the file LICENSE.
 Authors: Fabrizio Montesi
 -/
 
-import Cslib.Semantics.Lts.Basic
+import Cslib.Foundations.Semantics.Lts.Basic
 
+/-- A Deterministic Finite-State Automaton (DFA) consists of a labelled transition function
+`tr` over a finite set of states. It has a starting state `start` and a finite
+set of accepting states `accept`. -/
 structure Dfa (State : Type _) (Label : Type _) where
-  -- The transition system of the automaton
-  lts : Lts State Label
+  -- The transition function of the automaton
+  tr : State → Label → State
   -- Start state
   start : State
   -- Accept states
   accept : Finset State
   -- The automaton is finite-state
-  finite_state : lts.FiniteState
-  -- The automaton is deterministic
-  deterministic : lts.Deterministic
+  finite_state : Finite State
+
+namespace Dfa
+
+/-- `Dfa` is a special case of `Lts`. -/
+@[grind]
+def toLts (dfa : Dfa State Label) : Lts State Label :=
+  Lts.mk (fun s1 μ s2 => dfa.tr s1 μ = s2)
+
+instance : Coe (Dfa State Label) (Lts State Label) where
+  coe := toLts
+
+/-- The LTS induced by a DFA is deterministic. -/
+@[grind]
+theorem toLts_deterministic (dfa : Dfa State Label) : dfa.toLts.Deterministic := by
+  intro s1 μ s2 s3 htr2 htr3
+  by_cases heq : s2 = s3
+  case pos => exact heq
+  case neg =>
+    cases htr2
+    cases htr3
+    rfl
+
+/-- The LTS induced by a DFA is finite-state. -/
+@[grind]
+theorem toLts_finiteState (dfa : Dfa State Label) : dfa.toLts.FiniteState :=
+  dfa.finite_state
+
+/-- A DFA accepts a trace if there is a multi-step accepting derivative with that trace from
+the start state. -/
+@[grind]
+def Accepts (dfa : Dfa State Label) (μs : List Label) :=
+  ∃ s ∈ dfa.accept, dfa.toLts.MTr dfa.start μs s
+
+/-- The language of a DFA is the set of traces that it accepts. -/
+@[grind]
+def language (dfa : Dfa State Label) : Set (List Label) :=
+  fun μs => dfa.Accepts μs
+
+/-- A trace is accepted by a DFA iff it is in the language of the DFA. -/
+@[grind]
+theorem accepts_mem_language (dfa : Dfa State Label) (μs : List Label) :
+  dfa.Accepts μs ↔ μs ∈ dfa.language := by
+  constructor <;> intro h
+  case mp =>
+    exact h
+  case mpr =>
+    rcases h with ⟨s, h1, h2⟩
+    exists s
+
+end Dfa
